Translate liveness statement from TLA formalization

hpaxos_liveness.thy
@@ -2,48 +2,68 @@ theory hpaxos_liveness
 imports Main hpaxos hpaxos_safety
 begin
 
-fun Termination_lrn :: "(nat \<Rightarrow> State) \<Rightarrow> Learner \<Rightarrow> bool" where
-  "Termination_lrn f l = (\<exists>n :: nat. \<exists>b :: Ballot. decision (f n) l b \<noteq> {})"
+(*
+WF_vars(\E v \in Value : LearnerDecide(L, b, v))
+*)
 
-fun Termination :: "(nat \<Rightarrow> State) \<Rightarrow> bool" where
-  "Termination f = 
-     (\<forall>l :: Learner.  
-        (\<exists>Q :: Acceptor set. Q \<subseteq> {x . is_safe x} \<and> TrustLive l Q) \<longrightarrow>
-        Termination_lrn f l)"
+(* Send1a is always enabled.
+fun Send1a_Enabled :: "Ballot \<Rightarrow> State \<Rightarrow> bool" where
+  "Send1a_Enabled b st = True"
+*)
 
-(*Extract consecutive runs of given lengths from a stream*)
-fun sequence_of_runs :: "nat \<Rightarrow> nat list \<Rightarrow> (nat \<Rightarrow> 'a) \<Rightarrow> ('a list) list" where
-  "sequence_of_runs start [] f = []" |
-  "sequence_of_runs start (len # lens) f = 
-    map f [start ..< start + len] # sequence_of_runs (start + len) lens f"
+fun Process1a_Enabled :: "Acceptor \<Rightarrow> PreMessage \<Rightarrow> State \<Rightarrow> bool" where
+  "Process1a_Enabled a m st = (
+    type m = T1a \<and>
+    Recv_acc st a m
+  )"
 
-lemma sequence_of_runs_length_invar:
-  shows "\<forall> start1 start2 f1 f2. 
-           length (sequence_of_runs start1 lens f1) 
-           = length (sequence_of_runs start2 lens f2)"
-proof (induction lens; simp) qed
+fun Process1b_Enabled :: "Acceptor \<Rightarrow> PreMessage \<Rightarrow> State \<Rightarrow> bool" where
+  "Process1b_Enabled a m st = (
+    type m = T1b
+    \<and> Recv_acc st a m
+  )"
 
-theorem sequence_of_runs_length:
-  shows "length (sequence_of_runs start lens f) = length lens"
-proof (induction lens)
-  case Nil
-  then show ?case by simp
-next
-  case (Cons a lens)
-  then show ?case 
-    by (metis length_Cons sequence_of_runs.simps(2) sequence_of_runs_length_invar)
-qed
+(* Process1bLearnerLoop is always enabled.
+fun Process1bLearnerLoop_Enabled :: "Acceptor \<Rightarrow> State \<Rightarrow> bool" where
+  "Process1bLearnerLoop_Enabled a st = True"
+*)
 
+fun LearnerRecv_Enabled :: "Learner \<Rightarrow> PreMessage \<Rightarrow> State \<Rightarrow> bool" where
+  "LearnerRecv_Enabled l m st = (
+    Recv_lrn st l m
+  )"
 
+fun LearnerDecide_Enabled :: "Learner \<Rightarrow> Ballot \<Rightarrow> Value \<Rightarrow> State \<Rightarrow> bool" where
+  "LearnerDecide_Enabled l b v st = ChosenIn st l b v"
 
-fun runs_assumption :: "(State list) list \<Rightarrow> bool" where
-  "runs_assumption runs = True"
-
-fun network_assumption :: "(nat \<Rightarrow> State) \<Rightarrow> bool" where
-"network_assumption f = 
-    (\<exists>start lens. length lens = 13 \<and> (\<forall>i<13. lens ! i > 0) \<and> 
-                  runs_assumption (sequence_of_runs start lens f))"
+fun WF :: "(State \<Rightarrow> bool) \<Rightarrow> (State \<Rightarrow> State \<Rightarrow> bool) \<Rightarrow> (nat \<Rightarrow> State) \<Rightarrow> bool" where
+  "WF p_Enabled p f = (
+    \<forall>i. (\<forall>j \<ge> i. p_Enabled (f j)) \<longrightarrow> (\<exists>j \<ge> i. p (f j) (f (j + 1)))
+  )"
 
 
+fun Liveness :: "(nat \<Rightarrow> State) \<Rightarrow> bool" where
+  "Liveness f = (
+    \<forall> L :: Learner. \<forall> b :: Ballot. \<forall>Q :: Acceptor set. is_quorum Q \<longrightarrow>
+    (\<forall>a \<in> Q. is_safe a) \<and> (
+    TrustLive L Q \<longrightarrow> (
+    ((\<forall>m :: PreMessage. type m = T1a \<longrightarrow> bal m < b) \<and>
+     (\<forall>c :: Ballot. c > b \<longrightarrow> (\<forall>j. \<not> (Send1a c (f j) (f (1 + j))))) \<and>
+     (WF (\<lambda>x. True) (Send1a b) f) \<and>
+     (\<forall>m :: PreMessage. B m b \<longrightarrow> (\<forall>a \<in> Q. WF (Process1a_Enabled a m) (Process1a a m) f)) \<and>
+     (\<forall>m :: PreMessage. B m b \<longrightarrow> (\<forall>a \<in> Q. WF (Process1b_Enabled a m) (Process1b a m) f)) \<and>
+     (\<forall>a \<in> Q. WF (\<lambda>x. True) (Process1bLearnerLoop a) f) \<and>
+     (\<forall>m :: PreMessage. B m b \<longrightarrow> WF (LearnerRecv_Enabled L m) (LearnerRecv L m) f) \<and>
+     (WF (\<lambda>st. \<exists> v :: Value. LearnerDecide_Enabled L b v st) 
+         (\<lambda>st st2. \<exists> v :: Value. LearnerDecide L b v st st2) f)
+    ) \<longrightarrow> (\<exists>j. \<exists> BB :: Ballot . decision (f j) L BB \<noteq> {})
+  )))"
+
+
+
+theorem LivenessResult :
+  assumes "Spec f"
+  shows "Liveness f"
+sorry
 
 end
